prove memory safety for Division

code/experimental/rsa/Division.fst
@@ -17,30 +17,56 @@ type lbignum (len:U32.t) =
 
 type bnlen = (l:U32.t{U32.v l > 0 /\ U32.v l <= 8192})
 
+type rem_state (rLen:bnlen) (modLen:bnlen) = lbignum U32.(rLen +^ modLen +^ modLen +^ rLen)
+
+let get_r_i #r #m (st:rem_state r m) : lbignum r = Buffer.sub st 0ul r
+let get_mod #r #m (st:rem_state r m) : lbignum m = Buffer.sub st r m
+let get_mod_1 #r #m (st:rem_state r m) : lbignum m = Buffer.sub st U32.(r +^ m) m
+let get_tmp #r #m (st:rem_state r m) :lbignum r = Buffer.sub st U32.(r +^ m +^ m) r
+
+let rem_state_inv r m (st:rem_state r m) = 
+           let r_i = get_r_i st in
+           let tmp = get_tmp st in
+           let mod = get_mod st in
+           let mod_1 = get_mod_1 st in
+           let r = frameOf r_i in
+	     r == frameOf mod /\
+	     r == frameOf mod_1 /\
+	     r == frameOf tmp /\
+	     disjoint r_i tmp /\
+	     disjoint r_i mod /\
+	     disjoint r_i mod_1 /\ 
+	     disjoint tmp mod /\ 
+	     disjoint tmp mod_1 /\ 
+       	 disjoint mod mod_1 
+
+
+let rem_state_st_inv (rLen:bnlen) (modLen:bnlen) (st:rem_state rLen modLen) (h:FStar.HyperStack.mem) = 
+	     rem_state_inv rLen modLen st /\ live h st
+
 val remainder_loop:
     rLen:bnlen ->
     modLen:bnlen ->
-    r_i:lbignum rLen ->
-    mod:lbignum modLen ->
-    count:U32.t -> Stack unit
-        (requires (fun h -> live h r_i /\ live h mod))
-	    (ensures (fun h0 _ h1 -> live h0 r_i /\ live h0 mod /\
-            live h1 r_i /\ live h1 mod /\ modifies_2 mod r_i h0 h1))
+    count:U32.t ->
+    st:rem_state rLen modLen -> Stack unit
+        (requires (fun h -> rem_state_st_inv rLen modLen st h))
+	    (ensures (fun h0 _ h1 -> rem_state_st_inv rLen modLen st h1 /\
+			   modifies_1 st h0 h1))
 
-let rec remainder_loop rLen modLen r_i mod count =
-    push_frame();
-    let mod1 = create 0uL modLen in
-    let tmp = create 0uL rLen in
-    (if U32.(count >^ 0ul) then begin
+let rec remainder_loop rLen modLen count st =
+    let r_i = get_r_i st in
+    let mod = get_mod st in
+    let mod1 = get_mod_1 st in
+    let tmp = get_tmp st in
+    if U32.(count >^ 0ul) then begin
         rshift1 modLen mod mod1;
         let tmp_b = isMore modLen rLen mod r_i in
         (if not tmp_b then begin
-		    sub rLen modLen r_i mod tmp; 
+		    sub rLen modLen r_i mod tmp;
             blit tmp 0ul r_i 0ul rLen end);
-        blit mod1 0ul mod 0ul modLen;    
-        remainder_loop rLen modLen r_i mod U32.(count -^ 1ul)
-        end);
-    pop_frame()
+        blit mod1 0ul mod 0ul modLen;
+        remainder_loop rLen modLen U32.(count -^ 1ul) st
+        end
 
 (* res = a % mod *)
 val remainder:
@@ -49,21 +75,32 @@ val remainder:
     resLen:bnlen{U32.v resLen <= U32.v modLen} ->
     diffBits:U32.t{U32.v diffBits = op_Multiply 64 (U32.v aLen - U32.v modLen)} ->
     a:lbignum aLen ->
-    mod:lbignum modLen ->
-    res:lbignum resLen -> Stack unit
+    mod:lbignum modLen{disjoint mod a} ->
+    res:lbignum resLen{disjoint res a /\ disjoint res mod} -> Stack unit
 	    (requires (fun h -> live h a /\ live h mod /\ live h res))
 	    (ensures (fun h0 _ h1 -> live h0 a /\ live h0 mod /\  live h0 res /\
             live h1 a /\ live h1 mod /\ live h1 res /\ modifies_1 res h0 h1))
+
+#set-options "--z3rlimit 150"
 
 let remainder aLen modLen resLen diffBits a mod res =
     push_frame();
     let modk = U32.(diffBits /^ 64ul) in
     let mod1Len = U32.(modLen +^ modk +^ 1ul) in
-    let mod1 = create 0uL mod1Len in
-    lshift modLen mod diffBits mod1;
+    assume(U32.v mod1Len > 0 /\ U32.v mod1Len <= 8192);
     let a1Len = U32.(aLen +^ 1ul) in
-    let r0 = create 0uL a1Len in
-    blit a 0ul r0 0ul aLen;
-    remainder_loop a1Len mod1Len r0 mod1 diffBits;
-    blit r0 0ul res 0ul resLen;
+    assume(U32.v a1Len > 0 /\ U32.v a1Len <= 8192);
+    let mod1Len: bnlen = mod1Len in
+    let a1Len: bnlen = a1Len in
+    assert(U32.v a1Len = U32.v mod1Len);
+    let st : rem_state a1Len mod1Len = create 0uL U32.(a1Len +^ a1Len +^ mod1Len +^ mod1Len) in
+    let r_0 = get_r_i st in
+    let mod1 = get_mod st in
+
+    lshift modLen mod diffBits mod1;
+    blit a 0ul r_0 0ul aLen;
+
+    remainder_loop a1Len mod1Len diffBits st;
+
+    blit r_0 0ul res 0ul resLen;
     pop_frame()
